done/Iron/Language/Simple/Base.v
@@ -1,10 +1,8 @@
 
 Require Export Iron.Data.List.
 Require Export Iron.Data.Nat.
-
 Require Export Iron.Norm.List.
 Require Export Iron.Norm.
-
 Require Export Iron.Tactics.Rip2.
 Require Export Iron.Tactics.Case.
 Require Export Iron.Tactics.Nope.
@@ -15,7 +13,6 @@ Require Export Iron.Tactics.Down.
 Require Export Iron.Tactics.Rewrite.
 Require Export Iron.Tactics.Have.
 Require Export Iron.Tactics.LibTactics.
-
 Require Export Coq.Arith.Compare_dec.
 Require Import Coq.Logic.FunctionalExtensionality.
 
